Killed admits in Wordize.v

src/Assembly/Wordize.v
@@ -3,7 +3,7 @@ Require Import NArith PArith Ndigits Nnat NPow NPeano Ndec.
 Require Import Compare_dec Omega Bool.
 Require Import FunctionalExtensionality ProofIrrelevance.
 Require Import QhasmUtil QhasmEvalCommon.
-Require Import WordizeUtil Bounds List Listize.
+Require Import WordizeUtil Bounds List Listize Natize.
 
 Import EvalUtil ListNotations.
 
@@ -172,49 +172,235 @@ End ToWord.
 
 Section WordEq.
   Definition wordeq {ins outs} (n: nat) (f: Curried N N ins outs) :=
-    {g: Curried (word n) (word n) ins outs |
-    forall (x: list (word n)), length x = ins ->
+    {g: Curried (word n) (word n) ins outs | forall (x: list (word n)),
       (curriedToListF (wzero _) g) x =
         map (@NToWord n) ((curriedToListF 0%N f) (map (@wordToN n) x))}.
 
-  Definition wordeq_kill_arg: forall {n ins outs} (f: Curried N N (S ins) outs),
-    (forall x, wordeq n (f x)) -> wordeq n f.
-  Proof. Admitted.
+  Definition wordeq_kill_arg'' {m n w}
+      (f: Curried N N (S m) n)
+      (g: forall x, wordeq w (f x)): Curried (word w) (word w) (S m) n :=
+    fun x => proj1_sig (g (wordToN x)).
 
-  Definition wordeq_break_cons: forall {n m} (a: N) (b: list N),
-    @wordeq O 1 n [a] ->
-    @wordeq O (S m) n b ->
-    @wordeq O (S (S m)) n (cons a b).
-  Proof. Admitted.
+  Lemma wordToN_zero: forall w, wordToN (wzero w) = 0%N.
+  Proof.
+    intros.
+    unfold wzero; rewrite wordToN_nat.
+    rewrite wordToNat_natToWord_idempotent; simpl; intuition.
+    apply Npow2_gt0.
+  Qed.
 
-  Definition wordeq_nil: forall n, @wordeq O O n [].
-  Proof. Admitted.
+  Lemma wordeq_kill_arg': forall {m n w: nat}
+        (f: Curried N N (S m) n)
+        (g: forall x : N, wordeq w (f x))
+        (x: list (word w)),
+    curriedToListF (wzero w) (wordeq_kill_arg'' f g) x =
+        map (NToWord w) (curriedToListF 0%N f (map (@wordToN w) x)).
+  Proof.
+    intros; unfold wordeq_kill_arg'', curriedToListF; simpl in *.
+    destruct (g _) as [f' p]; simpl.
+    pose proof (p (tl x)) as p'; clear p.
+    rewrite <- (wordToN_zero w).
+    replace (m - m) with O in * by omega.
+    rewrite map_nth.
+    unfold curriedToListF in p'.
+    replace (map (@wordToN w) (tl x)) with (tl (map (@wordToN w) x)) in p'.
+    replace (curriedToListF' (S m) (wzero w) f' x)
+        with (curriedToListF' m (wzero w) f' (tl x));
+        try rewrite p'; try clear f'; try clear f; try f_equal.
 
-  Definition wordeq_cut_let: forall {n outs} (x: N) (f: N -> list N),
-    @wordeq 1 outs n f -> @wordeq O 1 n [x] ->
-    @wordeq O outs n (Let_In x f).
-  Proof. Admitted.
+    - rewrite curriedToListF'_tl; try omega.
+      repeat f_equal; intuition.
+      rewrite wordToN_zero.
+      reflexivity.
 
-  Definition wordeq_let_const: forall {T n outs} (a: T) (f: T -> list N),
-    @wordeq O outs n (f a) -> @wordeq O outs n (Let_In a f).
-  Proof. Admitted.
+    - rewrite curriedToListF'_tl; try omega.
+      rewrite p'.
+      reflexivity.
 
-  Definition wordeq_debool_andb: forall {n outs} (a b: bool) (f: bool -> list N),
-    @wordeq O outs n (Let_In a (fun x => Let_In b (fun y => f (andb x y)))) ->
-    @wordeq O outs n (Let_In (andb a b) f).
-  Proof. Admitted.
+    - induction x; simpl; intuition.
+  Qed.
 
-  Definition wordeq_debool_ltb: forall {n outs} (x y: N) (f: bool -> list N),
-    @wordeq O outs n (f true) -> @wordeq O outs n (f false) ->
-    @wordeq O 1 n [x] -> @wordeq O 1 n [y] ->
-    @wordeq O outs n (Let_In (x <? y)%N f).
-  Proof. Admitted.
+  Definition wordeq_kill_arg {m n w} (f: Curried N N (S m) n):
+    (forall x, wordeq w (f x)) -> wordeq w f.
+  Proof.
+    refine (fun g => exist _ (wordeq_kill_arg'' f g) _).
+    apply wordeq_kill_arg'.
+  Defined.
 
-  Definition wordeq_debool_eqb: forall {n outs} (x y: N) (f: bool -> list N),
-    @wordeq O outs n (f true) -> @wordeq O outs n (f false) ->
-    @wordeq O 1 n [x] -> @wordeq O 1 n [y] ->
-    @wordeq O outs n (Let_In (x =? y)%N f).
-  Proof. Admitted.
+  Definition wordeq_break_cons: forall {m w} (a: N) (b: list N),
+    @wordeq O 1 w [a] ->
+    @wordeq O (S m) w b ->
+    @wordeq O (S (S m)) w (cons a b).
+  Proof.
+    intros m w a b n0 n1.
+    exists (@cons (word w) (hd (wzero w) (proj1_sig n0)) (proj1_sig n1)); intro x.
+    destruct n0 as [f0 p0].
+    destruct n1 as [f1 p1].
+    pose proof (p0 x) as p0'.
+    pose proof (p1 x) as p1'.
+
+    abstract (
+        unfold curriedToListF in *;
+        simpl in *;
+        rewrite p0', p1';
+        simpl; reflexivity).
+  Defined.
+
+  Definition wordeq_nil: forall w, @wordeq O O w [].
+  Proof. intro; exists []; abstract (intro; simpl; reflexivity). Qed.
+
+  Definition wordeq_cut_let: forall {outs w} (x: N) (f: N -> list N),
+    (x < Npow2 w)%N ->
+    (0 <= x)%N ->
+    @wordeq 1 outs w f -> @wordeq O 1 w [x] ->
+    @wordeq O outs w (Let_In x f).
+  Proof.
+    intros outs w x f B H n0 n1.
+    exists (Let_In (hd (wzero w) (proj1_sig n1)) (proj1_sig n0)); intro x0.
+
+    destruct n0 as [f0 p0].
+    destruct n1 as [f1 p1].
+    pose proof (p0 [NToWord w x]) as p0'.
+    pose proof (p1 x0) as p1'.
+
+    abstract (
+        unfold curriedToListF, Let_In in *;
+        simpl in *;
+        rewrite p1'; simpl;
+        rewrite p0'; simpl;
+        f_equal;
+        rewrite wordToN_NToWord;
+        intuition).
+  Qed.
+
+  Definition wordeq_let_const: forall {T outs w} (a: T) (f: T -> list N),
+    @wordeq O outs w (f a) -> @wordeq O outs w (Let_In a f).
+  Proof.
+    intros T outs w a f n0.
+    exists (proj1_sig n0); intro x0.
+    destruct n0 as [f0 p0].
+    pose proof (p0 x0) as p0'.
+    abstract (
+        simpl; rewrite p0'; unfold Let_In;
+        simpl; reflexivity).
+  Qed.
+
+  Definition wordeq_debool_andb: forall {outs w} (a b: bool) (f: bool -> list N),
+    @wordeq O outs w (Let_In a (fun x => Let_In b (fun y => f (andb x y)))) ->
+    @wordeq O outs w (Let_In (andb a b) f).
+  Proof.
+    intros T outs w a f n0.
+    exists (proj1_sig n0); intro x0.
+    destruct n0 as [f0 p0].
+    pose proof (p0 x0) as p0'.
+    abstract (
+        simpl; rewrite p0'; unfold Let_In;
+        simpl; reflexivity).
+  Qed.
+
+  Definition wordeq_debool_ltb: forall {outs w} (x y: N) (f: bool -> list N),
+    (x < Npow2 w)%N -> (y < Npow2 w)%N ->
+    (0 <= x)%N -> (0 <= y)%N ->
+    @wordeq O outs w (f true) -> @wordeq O outs w (f false) ->
+    @wordeq O 1 w [x] -> @wordeq O 1 w [y] ->
+    @wordeq O outs w (Let_In (x <? y)%N f).
+  Proof.
+    intros outs w a b f B0 B1 I0 I1 n0 n1 n2 n3.
+
+    exists (if ((wordToN (hd (wzero w) (curriedToListF (wzero w) (proj1_sig n2) [])))
+            <? wordToN (hd (wzero w) (curriedToListF (wzero w) (proj1_sig n3) [])))%N
+        then (proj1_sig n0) else (proj1_sig n1)); intro x.
+
+    destruct n0 as [f0 p0].
+    destruct n1 as [f1 p1].
+    destruct n2 as [f2 p2].
+    destruct n3 as [f3 p3].
+
+    pose proof (p0 x) as p0'.
+    pose proof (p1 x) as p1'.
+    pose proof (p2 x) as p2'.
+    pose proof (p3 x) as p3'.
+
+    abstract (
+        unfold Let_In; simpl;
+        rewrite p2, p3; simpl;
+        repeat rewrite wordToN_NToWord; try assumption;
+        destruct (a <? b)%N; try assumption).
+  Qed.
+
+  Lemma Ninj_eqb: forall w a b,
+      (a < Npow2 w)%N -> (b < Npow2 w)%N ->
+      (weqb (NToWord w a) (NToWord w b)) = (a =? b)%N.
+  Proof.
+    intros w a b B0 B1.
+    symmetry.
+    rewrite <- (wordToN_NToWord w a) at 1; try assumption.
+    rewrite <- (wordToN_NToWord w b) at 1; try assumption.
+    destruct (weq (NToWord w a) (NToWord w b)) as [e|e].
+
+    - rewrite e at 1.
+      apply weqb_true_iff in e; rewrite e.
+      repeat rewrite wordToN_NToWord; try assumption.
+      apply N.eqb_eq.
+      reflexivity.
+
+    - assert (a <> b) as H by (
+        intro H; rewrite H in e; apply e; reflexivity).
+      repeat rewrite wordToN_NToWord; try assumption.
+      replace (weqb _ _) with false.
+
+      + assert ((a =? b)%N <> true). {
+          intro H0.
+          rewrite N.eqb_eq in H0.
+          rewrite H0 in H.
+          apply H.
+          reflexivity.
+        }
+
+        induction (a =? b)%N; intuition.
+
+      + assert (weqb (NToWord w a) (NToWord w b) <> true). {
+          intro H0.
+          rewrite weqb_true_iff in H0.
+          rewrite H0 in e.
+          apply e.
+          reflexivity.
+        }
+
+        induction (weqb _ _); intuition.
+  Qed.
+
+  Definition wordeq_debool_eqb: forall {outs w} (x y: N) (f: bool -> list N),
+    (x < Npow2 w)%N -> (y < Npow2 w)%N ->
+    (0 <= x)%N -> (0 <= y)%N ->
+    @wordeq O outs w (f true) -> @wordeq O outs w (f false) ->
+    @wordeq O 1 w [x] -> @wordeq O 1 w [y] ->
+    @wordeq O outs w (Let_In (N.eqb x y) f).
+  Proof.
+    intros outs w a b f B0 B1 I0 I1 n0 n1 n2 n3.
+
+    exists (if (weqb
+            (hd (wzero w) (curriedToListF (wzero w) (proj1_sig n2) []))
+            (hd (wzero w) (curriedToListF (wzero w) (proj1_sig n3) [])))%N
+        then (proj1_sig n0) else (proj1_sig n1)); intro x.
+
+    destruct n0 as [f0 p0].
+    destruct n1 as [f1 p1].
+    destruct n2 as [f2 p2].
+    destruct n3 as [f3 p3].
+
+    pose proof (p0 x) as p0'.
+    pose proof (p1 x) as p1'.
+    pose proof (p2 x) as p2'.
+    pose proof (p3 x) as p3'.
+
+    abstract (
+        unfold Let_In; simpl;
+        rewrite p2, p3; simpl;
+        rewrite Ninj_eqb;
+        destruct (a =? b)%N;
+        assumption).
+  Qed.
 
 End WordEq.
 
@@ -225,8 +411,8 @@ Ltac standardize_wordeq :=
   | [|- @wordeq (S ?m) _ _ _] => apply wordeq_kill_arg; intro
   | [|- @wordeq O _ _ (Let_In true _)] => apply wordeq_let_const
   | [|- @wordeq O _ _(Let_In false _)] => apply wordeq_let_const
-  | [|- @wordeq O _ _ (Let_In (_ <? _)%Z _)] => apply wordeq_debool_ltb
-  | [|- @wordeq O _ _ (Let_In (_ =? _)%Z _)] => apply wordeq_debool_eqb
+  | [|- @wordeq O _ _ (Let_In (_ <? _)%N _)] => apply wordeq_debool_ltb
+  | [|- @wordeq O _ _ (Let_In (_ =? _)%N _)] => apply wordeq_debool_eqb
   | [|- @wordeq O _ _ (Let_In (andb _ _) _)] => apply wordeq_debool_andb
   | [|- @wordeq O _ _ (Let_In _ _)] => apply wordeq_cut_let
   | [|- @wordeq O _ _ (cons _ _)] => apply wordeq_break_cons
